StrataTest/Languages/Core/SMTEncoderTests.lean
@@ -80,7 +80,7 @@ info: "; f\n(declare-fun f (Int Int) Int)\n; x\n(declare-const x Int)\n(define-f
       config := { Env.init.exprEnv.config with
         factory :=
           Env.init.exprEnv.config.factory.push $
-          LFunc.mk "f" [] False [("m", LMonoTy.int), ("n", LMonoTy.int)] LMonoTy.int .none #[] .none [] []
+          LFunc.mk "f" [] false false [("m", LMonoTy.int), ("n", LMonoTy.int)] LMonoTy.int .none #[] .none [] []
       }
    }})
 
@@ -98,7 +98,7 @@ info: "; f\n(declare-fun f (Int Int) Int)\n; x\n(declare-const x Int)\n(define-f
       config := { Env.init.exprEnv.config with
         factory :=
           Env.init.exprEnv.config.factory.push $
-          LFunc.mk "f" [] False [("m", LMonoTy.int), ("n", LMonoTy.int)] LMonoTy.int .none #[] .none [] []
+          LFunc.mk "f" [] false false [("m", LMonoTy.int), ("n", LMonoTy.int)] LMonoTy.int .none #[] .none [] []
       }
    }})
 
